CookLevin/Complexity.lean
@@ -2,6 +2,7 @@ import Complexity.Complexity.MachineSemantics
 import Complexity.Complexity.TMDecider
 import Complexity.Complexity.TMEncoding
 import Complexity.Complexity.TMPrimitives
+import Complexity.Complexity.Deciders.SAT_TM
 import Complexity.NP.SAT.CookLevin
 
 set_option autoImplicit false
